spec: move counter Iris facts out of Justin Iris core

packages/zoe/spec/jessie_iris_lang.v
@@ -1,6 +1,6 @@
 From Coq Require Import List String ZArith.
 From iris.program_logic Require Export ectxi_language.
-Require Import jessie_lang jessie_justin jessie_counter.
+Require Import jessie_lang jessie_justin.
 
 Import ListNotations.
 Open Scope list_scope.
@@ -10,7 +10,6 @@ Open Scope Z_scope.
 Module JustinIris.
   Import Justin.
   Import JustinExec.
-  Import JessieCounterCase.
 
   Definition expr := core_expr.
   Definition val := Justin.val.
@@ -361,89 +360,4 @@ Module JustinIris.
     fill_item (BinOpLCtx EqStrictOp (CoreAllocObj [])) (CoreAllocObj []) =
       CoreBinop EqStrictOp (CoreAllocObj []) (CoreAllocObj []).
   Proof. reflexivity. Qed.
-
-  Definition counter_after_makeCounter : val :=
-    match fst (apply_prim empty_state "makeCounter" []) with
-    | CoreLit v => v
-    | _ => VUndefined
-    end.
-
-  Definition state_after_makeCounter : state :=
-    snd (apply_prim empty_state "makeCounter" []).
-
-  Definition entry_cap_after_makeCounter : option (val * state) :=
-    alloc_entry_cap state_after_makeCounter counter_after_makeCounter.
-
-  Definition exit_cap_after_makeCounter : option (val * state) :=
-    alloc_exit_cap state_after_makeCounter counter_after_makeCounter.
-
-  Example entry_cap_get_incr_atomic :
-    match entry_cap_after_makeCounter with
-    | Some (cap, σ) =>
-        base_step (CoreGet (CoreLit cap) "incr") σ []
-          (CoreLit (VPrim (counter_incr_name 0%nat))) σ []
-    | None => False
-    end.
-  Proof.
-    vm_compute.
-    econstructor.
-    - reflexivity.
-    - reflexivity.
-  Qed.
-
-  Example entry_cap_get_decr_missing_atomic :
-    match entry_cap_after_makeCounter with
-    | Some (cap, σ) =>
-        base_step (CoreGet (CoreLit cap) "decr") σ []
-          (CoreLit VUndefined) σ []
-    | None => False
-    end.
-  Proof.
-    vm_compute.
-    econstructor.
-    - reflexivity.
-    - reflexivity.
-  Qed.
-
-  Example entry_cap_call_incr_atomic :
-    match entry_cap_after_makeCounter with
-    | Some (_, σ) =>
-        base_step (CoreApp (CoreLit (VPrim (counter_incr_name 0%nat))) []) σ []
-          (CoreLit (VJson (JNum 1))) (store_cell σ 0%nat 1) []
-    | None => False
-    end.
-  Proof.
-    vm_compute.
-    econstructor.
-    - reflexivity.
-    - reflexivity.
-  Qed.
-
-  Example exit_cap_get_incr_missing_atomic :
-    match exit_cap_after_makeCounter with
-    | Some (cap, σ) =>
-        base_step (CoreGet (CoreLit cap) "incr") σ []
-          (CoreLit VUndefined) σ []
-    | None => False
-    end.
-  Proof.
-    vm_compute.
-    econstructor.
-    - reflexivity.
-    - reflexivity.
-  Qed.
-
-  Example exit_cap_call_decr_atomic :
-    match exit_cap_after_makeCounter with
-    | Some (_, σ) =>
-        base_step (CoreApp (CoreLit (VPrim (counter_decr_name 0%nat))) []) σ []
-          (CoreLit (VJson (JNum (-1)))) (store_cell σ 0%nat (-1)) []
-    | None => False
-    end.
-  Proof.
-    vm_compute.
-    econstructor.
-    - reflexivity.
-    - reflexivity.
-  Qed.
 End JustinIris.
